Add sigT_wfo back

nola/util/wfo.v
@@ -2,6 +2,7 @@
 
 From nola Require Import prelude.
 From stdpp Require Export well_founded.
+Import EqNotations.
 
 (** ** [wfo]: Type with a well-founded order *)
 
@@ -36,3 +37,37 @@ Lemma lt_wf : wf lt.
 Proof. apply well_founded_ltof. Qed.
 
 Canonical nat_wfo := Wfo nat lt lt_wf.
+
+(** ** Equip [sigT] with the lexicographic order *)
+
+Section sigT_wfo.
+  Context {A : wfo} (F : A → wfo).
+
+  (** Lexicographic strict and reflexive order for [sigT] *)
+  Definition sigT_lt (p q : sigT F) : Prop :=
+    projT1 p ≺ projT1 q  ∨
+    ∃ eq : projT1 p = projT1 q, rew eq in projT2 p ≺ projT2 q.
+
+  (** Lemma for [sigT_lt_wf] *)
+  Lemma sigT_lt_wf_pre a
+    (IH : ∀ a', a' ≺ a → ∀ b , Acc sigT_lt (existT a' b)) :
+    ∀ b , Acc wfo_lt b → Acc sigT_lt (existT a b).
+  Proof.
+    fix FIX 2. move=> b Accb. apply Acc_intro=> [[a' b']] [|]/=.
+    - move=> a'a. apply (IH _ a'a).
+    - move=> [?+]. subst. simpl_eq=> b'b. apply (FIX _ (Acc_inv Accb b'b)).
+  Qed.
+
+  (** [sigT_lt] is well-founded *)
+  Lemma sigT_lt_wf : wf sigT_lt.
+  Proof.
+    move=> [a b]. move: a (wfo_lt_wf a) b. fix FIX 2. move=> a Acca b.
+    apply Acc_intro=> [[a' b']] [|]/=.
+    - move=> a'a. apply (FIX _ (Acc_inv Acca a'a)).
+    - move=> [?+]. subst. simpl_eq=> b'b.
+      apply sigT_lt_wf_pre; [|exact (wfo_lt_wf b')].
+      clear dependent b b'=> a' a'a b. apply (FIX _ (Acc_inv Acca a'a)).
+  Qed.
+
+  Canonical sigT_wfo := Wfo (sigT F) sigT_lt sigT_lt_wf.
+End sigT_wfo.
